books/kestrel/std/system/definedp-tests.lisp
@@ -1,0 +1,41 @@
+; Standard System Library
+;
+; Copyright (C) 2019 Kestrel Institute (http://www.kestrel.edu)
+;
+; License: A 3-clause BSD license. See the LICENSE file distributed with ACL2.
+;
+; Author: Alessandro Coglio (coglio@kestrel.edu)
+
+;;;;;;;;;;;;;;;;;;;;;;;;;;;;;;;;;;;;;;;;;;;;;;;;;;;;;;;;;;;;;;;;;;;;;;;;;;;;;;;;
+
+(in-package "ACL2")
+
+(include-book "definedp")
+
+(include-book "misc/assert" :dir :system)
+(include-book "misc/eval" :dir :system)
+
+;;;;;;;;;;;;;;;;;;;;;;;;;;;;;;;;;;;;;;;;;;;;;;;;;;;;;;;;;;;;;;;;;;;;;;;;;;;;;;;;
+
+(assert! (definedp 'not (w state)))
+
+(assert! (not (definedp 'cons (w state))))
+
+(must-succeed*
+ (defun f (x) x)
+ (assert! (definedp 'f (w state))))
+
+(must-succeed*
+ (defstub f (*) => *)
+ (assert! (not (definedp 'f (w state)))))
+
+(must-succeed*
+ (encapsulate
+   (((f *) => *))
+   (local (defun f (x) x))
+   (defthm th (equal (f x) x)))
+ (assert! (not (definedp 'f (w state)))))
+
+(must-succeed*
+ (defchoose f x (y) (equal x y))
+ (assert! (not (definedp 'f (w state)))))
