books/kestrel/utilities/system/world-queries-tests.lisp
@@ -15,31 +15,6 @@
 
 ;;;;;;;;;;;;;;;;;;;;;;;;;;;;;;;;;;;;;;;;;;;;;;;;;;;;;;;;;;;;;;;;;;;;;;;;;;;;;;;;
 
-(assert! (definedp 'not (w state)))
-
-(assert! (not (definedp 'cons (w state))))
-
-(must-succeed*
- (defun f (x) x)
- (assert! (definedp 'f (w state))))
-
-(must-succeed*
- (defstub f (*) => *)
- (assert! (not (definedp 'f (w state)))))
-
-(must-succeed*
- (encapsulate
-   (((f *) => *))
-   (local (defun f (x) x))
-   (defthm th (equal (f x) x)))
- (assert! (not (definedp 'f (w state)))))
-
-(must-succeed*
- (defchoose f x (y) (equal x y))
- (assert! (not (definedp 'f (w state)))))
-
-;;;;;;;;;;;;;;;;;;;;;;;;;;;;;;;;;;;;;;;;;;;;;;;;;;;;;;;;;;;;;;;;;;;;;;;;;;;;;;;;
-
 (assert! (definedp+ 'not (w state)))
 
 (assert! (not (definedp+ 'cons (w state))))
